ApcOptimizer/Implementation/OptimizerPasses/Reencode.lean
@@ -1,4 +1,3 @@
-import ApcOptimizer.Implementation.OptimizerPasses.OldVariableBased.Reencode
 import ApcOptimizer.Implementation.OptimizerPasses.DomainBatch
 import ApcOptimizer.Implementation.OptimizerPasses.DomainFold
 
